Add crashes to interpreter correctness
Using the same invariant for crashes is definitely not general enough,
but let's get through some simpler stuff before constructing an example
where we need a bonafide crash invariant.

Shallow/Interpret.v
@@ -30,35 +30,75 @@ Section Interpreter.
   Notation exec1 := (exec step1).
   Notation exec2 := (exec step2).
 
+  (* TODO: in general, it might not be the case that crash states line up with
+  abstract states as desired; there might be states that are only exposed by
+  recovery and that are then patched up during recovery. *)
+  Definition res_abstraction T (r: Result State1 T) : Result State2 T :=
+    match r with
+    | Finished v state => Finished v (abstraction state)
+    | Crashed state => Crashed (abstraction state)
+    end.
+
+  (* TODO: similar problem here, where there might be a weaker crash
+  invariant *)
+  Definition res_invariant T (r: Result State1 T) : Prop :=
+    match r with
+    | Finished _ state => invariant state
+    | Crashed state => invariant state
+    end.
+
   Hint Constructors exec.
 
   Theorem interpret_exec :
-    (forall T (op: opT2 T) state v state',
-        invariant state ->
-        exec1 (op_impl op) state (Finished v state') ->
-        step2 op (abstraction state) v (abstraction state') /\ invariant state') ->
-    forall T (p: prog2 T) state v state',
+    (* every operation is implemented according to the step semantics of the
+    spec language *)
+    forall (Hop_ok: forall T (op: opT2 T) state v state',
+          invariant state ->
+          exec1 (op_impl op) state (Finished v state') ->
+          step2 op (abstraction state) v (abstraction state') /\ invariant state')
+      (* every implementation crashes in states that are abstractly either the
+        pre state or the post state
+
+        TODO: this is too strong, we only need this property after a crash
+        transform and recovery; the intermediate states can satisfy some weaker
+        crash invariant
+       *)
+      (Hop_crash: forall T (op: opT2 T) state state',
+          invariant state ->
+          exec1 (op_impl op) state (Crashed state') ->
+          (abstraction state' = abstraction state \/
+           exists v, step2 op (abstraction state) v (abstraction state')) /\
+          invariant state'),
+    forall T (p: prog2 T) state r,
       invariant state ->
-      exec1 (interpret p) state (Finished v state') ->
-      exec2 p (abstraction state) (Finished v (abstraction state')) /\
-      invariant state'.
+      exec1 (interpret p) state r ->
+      exec2 p (abstraction state) (res_abstraction r) /\
+      res_invariant r.
   Proof.
     induction p; simpl; intros.
-    eapply H in H1; eauto.
-    intuition eauto.
-
-    inv_exec; eauto.
-
-    inv_exec.
-    match goal with
-    | [ Hexec: exec1 (interpret p) _ _ |- _ ] =>
-      eapply IHp in Hexec; eauto; safe_intuition
-    end.
-    match goal with
-    | [ Hexec: exec1 (interpret (p0 _)) _ _ |- _ ] =>
-      eapply H0 in Hexec; eauto; safe_intuition
-    end.
-    intuition eauto.
+    - destruct r; simpl.
+      + eapply Hop_ok in H0; eauto.
+        intuition eauto.
+      + eapply Hop_crash in H0; intuition eauto;
+          repeat deex;
+          eauto.
+        replace (abstraction state0); eauto.
+    - inv_exec; simpl; eauto.
+    - inv_exec.
+      + match goal with
+        | [ Hexec: exec1 (interpret p) _ _ |- _ ] =>
+          eapply IHp in Hexec; simpl in *; eauto; safe_intuition
+        end.
+        match goal with
+        | [ Hexec: exec1 (interpret (p0 _)) _ _ |- _ ] =>
+          eapply H in Hexec; eauto; safe_intuition
+        end.
+        intuition eauto.
+      + match goal with
+        | [ Hexec: exec1 (interpret p) _ _ |- _ ] =>
+          eapply IHp in Hexec; simpl in *; eauto; safe_intuition
+        end.
+        intuition eauto.
   Qed.
 
 End Interpreter.
